{
 "cells": [
  {
   "cell_type": "markdown",
   "metadata": {},
   "source": [
    "$p165.3.(1)$"
   ]
  },
  {
   "cell_type": "markdown",
   "metadata": {},
   "source": [
    "$设x=t^k,代入方程得到k(k-1)+k-1=0,所以k_1=1,k_2=-1,所以方程通解为x=c_1t+c_2\\frac{1}{t}$"
   ]
  },
  {
   "cell_type": "markdown",
   "metadata": {},
   "source": [
    "$(2)$"
   ]
  },
  {
   "cell_type": "markdown",
   "metadata": {},
   "source": [
    "$设x=t^k,带入方程得到k(k-1)-4k+6=0解得k_1=2,k_2=3,所以方程t^2x''-4tx'+6x=0的通解为x=c_1t^2+c_2t^3$"
   ]
  },
  {
   "cell_type": "markdown",
   "metadata": {},
   "source": [
    "$有方程组t^2c'_1(t)+t^3c'_2(t)=0和2tc'_1(t)+3t^2c'_2(t)=\\frac{1}{t}$"
   ]
  },
  {
   "cell_type": "markdown",
   "metadata": {},
   "source": [
    "$解得c'_1(t)=\\frac{-1}{t^2},c'_2(t)=\\frac{1}{t^3},所以方程的通解为x=c_1t^2+c_2t^3+\\frac{t}{2}$"
   ]
  },
  {
   "cell_type": "markdown",
   "metadata": {
    "collapsed": true
   },
   "source": [
    "# <font color='red'>A  8/11"
   ]
  },
  {
   "cell_type": "code",
   "execution_count": null,
   "metadata": {
    "collapsed": true
   },
   "outputs": [],
   "source": []
  }
 ],
 "metadata": {
  "kernelspec": {
   "display_name": "SageMath 7.3",
   "language": "",
   "name": "sagemath"
  },
  "language_info": {
   "codemirror_mode": {
    "name": "ipython",
    "version": 2
   },
   "file_extension": ".py",
   "mimetype": "text/x-python",
   "name": "python",
   "nbconvert_exporter": "python",
   "pygments_lexer": "ipython2",
   "version": "2.7.10"
  }
 },
 "nbformat": 4,
 "nbformat_minor": 0
}
