{
 "cells": [
  {
   "cell_type": "markdown",
   "metadata": {},
   "source": [
    "# homework3\n",
    "**P61**  \n",
    "**2.solve following equation**  \n",
    "**(8)$(x+2y)\\mathrm d x+x\\mathrm d y=0$**  \n",
    "**answer:**suppose $\\frac{y}{x}=t$  \n",
    "so $\\mathrm d y=x\\mathrm d t+t\\mathrm d x$  \n",
    "both sides of the equation multiply $\\frac{1}{x}$ and substitute $\\frac{y}{x}$ with $t$  \n",
    "\\begin{align}\n",
    "(1+2\\frac{y}{x})\\mathrm d x+\\mathrm d y&=0\\\\\n",
    "(1+2t)\\mathrm d x+x\\mathrm d t+t\\mathrm d x&=0\\\\\n",
    "(1+3t)\\mathrm d x+x\\mathrm d t&=0\\\\\n",
    "\\frac{\\mathrm d x}{x}&=-\\frac{\\mathrm d t}{1+3t}\\\\\n",
    "\\mathrm{ln} x&=-\\frac{1}{3}\\mathrm{ln}(1+3t)+c\\\\\n",
    "x^3&=c\\frac{1}{1+3t}\n",
    "\\end{align}\n",
    "substitute $t$ with $\\frac{y}{x}$,we got  \n",
    "\\begin{align}\n",
    "x^3&=c\\frac{1}{1+\\frac{3y}{x}}\\\\\n",
    "y&=\\frac{c}{3x^2}-\\frac{x}{3}\\\\\n",
    "\\end{align}\n",
    "that is the solution    \n",
    "**(9)$[xcos(x+y)+sin(x+y)]\\mathrm d x+xcos(x+y)\\mathrm d y=0$**  \n",
    "**answer:**\n",
    "\\begin{align}\n",
    "[xcos(x+y)+sin(x+y)]\\mathrm d x+xcos(x+y)\\mathrm d y&=0\\\\\n",
    "xcos(x+y)(\\mathrm d x+\\mathrm d y)+sin(x+y)\\mathrm d x&=0\\\\\n",
    "xcos(x+y)\\mathrm d (x+y)+sin(x+y)\\mathrm d x&=0\\\\\n",
    "x\\mathrm d (sin(x+y))+sin(x+y)\\mathrm d x&=0\\\\\n",
    "\\mathrm d(xsin(x+y))&=0\\\\\n",
    "xsin(x+y)&=c\n",
    "\\end{align}\n",
    "so $xsin(x+y)=c$ is the solution  \n",
    "**(10)$(ycosx-xsinx)\\mathrm d x+(ysinx+xcosx)\\mathrm d y=0$**  \n",
    "**answer:**$M=ycosx-xsinx$,$N=ysinx+xcosx$  \n",
    "$\\frac{\\partial M}{\\partial y}\\neq\\frac{\\partial N}{\\partial x}$  \n",
    "because $$\\frac{\\frac{\\partial M}{\\partial y}-\\frac{\\partial N}{\\partial x}}{-M}=1$$  \n",
    "the integral factor is $\\mu=e^{\\int\\mathrm d y}=e^y$  \n",
    "both sides of the equation multiply $\\mu$  \n",
    "$e^y(ycosx-xsinx)\\mathrm d x+e^y(ysinx+xcosx)\\mathrm d y=0$  \n",
    "this is an exact ODE,the solution is  \n",
    "$\\int {e^y(ycosx-xsinx)\\mathrm d x}+\\int{(N-\\frac{\\partial}{\\partial y}\\int{e^y(ysinx+xcosx)\\mathrm d y)}}=0$  \n",
    "that is $e^ysinx(y-1)+e^ycosx=c$  \n",
    "**(11)$x(4y\\mathrm d x+2x\\mathrm d y)+y^3(3y\\mathrm d x+5x\\mathrm d y)=0$**  \n",
    "**answer:**both sides of the equation times $x^2y$  \n",
    "$(4x^3y^2\\mathrm d x+2x^4y\\mathrm d y)+(3x^2y^5\\mathrm d x+5x^3y^4\\mathrm d y)=0$  \n",
    "$\\mathrm d (x^4y^2)+\\mathrm d (x^3y^5)=0$  \n",
    "so the solution is $x^4y^2+x^3y^5=c$  \n",
    "**4.suppose $f(x,y)$ and $\\frac{\\partial f}{\\partial y}$ are continuous,certifacate that the necessary and suffcient condition of that the equation $\\mathrm d y-f(x,y)\\mathrm d x=0$ is a liner differential equation is that the euqation has an integral factor which only depends on $x$.**  \n",
    "**answer:**  \n",
    "necessary:if the equation is a liner differential equation,it will be\n",
    "$\\frac{\\mathrm d y}{\\mathrm d x}=P(x)y+Q(x)$  \n",
    "this equation has the integral factor:$\\mu(x)=e^{-\\int{P(x)\\mathrm d x}}$,and $\\mu(x)$ only depends on x  \n",
    "sufficent:if the euqation has the integral factor $\\mu(x)$ which only depends on $x$,  \n",
    "the equation $\\mu(x)\\mathrm d y-\\mu(x)f(x,y)\\mathrm d x=0$ is an exact ODE.  \n",
    "so $\\frac{\\partial(-\\mu(x)f(x,y))}{\\partial y}=\\frac{\\mathrm d (\\mu(x))}{\\mathrm d x}$,\n",
    "$\\frac{\\partial f}{\\partial y}=-\\frac{\\mu^\\prime(x)}{\\mu(x)}$  \n",
    "$f=-\\int{\\frac{\\mu^\\prime(x)}{\\mu(x)}\\mathrm d y}+Q(x)=-\\frac{\\mu^\\prime(x)}{\\mu(x)}y+Q(x)=P(x)y+Q(x)$  \n",
    "so the equation can be change into a first order linear equation.  \n",
    "**8.solve the integral factor of the bernoulli equation **  \n",
    "**answer:**the form of the bernoulli equation is $\\frac{\\mathrm d y}{\\mathrm d x}=P(x)y+Q(x)y^n,y\\neq0$  \n",
    "both sides of the equation multiply $\\frac{1}{y^n}$,suppose $z=\\frac{1}{y^{n-1}}$    \n",
    "$\\frac{\\mathrm d z}{\\mathrm d x}=(1-n)P(x)z+(1-n)Q(x)$  \n",
    "this equation has the integral factor:$\\mu=e^{\\int{-(1-n)P(x)\\mathrm d x}}=e^{(n-1)\\int{P(x)\\mathrm d x}}$  \n",
    "so the integral factor of the original equation is $\\mu=e^{(n-1)\\int{P(x)\\mathrm d x}}$  \n",
    "**P69**  \n",
    "**1.solve following equation**  \n",
    "**(1)$x(\\frac{\\mathrm d y}{\\mathrm d x})^3=1+\\frac{\\mathrm d y}{\\mathrm d x}$**  \n",
    "**answer:**suppose $\\frac{\\mathrm d y}{\\mathrm d x}=p=\\frac{1}{t}$  \n",
    "so $x(\\frac{1}{t})^3=1+\\frac{1}{t}$,$x=(1+\\frac{1}{t})t^3=t^3+t^2$ then\n",
    "\\begin{align}\n",
    "y&=\\int{p\\mathrm d x}+c\\\\\n",
    "&=\\int{\\frac{1}{t}\\mathrm d (t^3+t^2)}+c\\\\\n",
    "&=\\int{(3t+2)\\mathrm d t}+c\\\\\n",
    "&=\\frac{3}{2}t^2+2t+c\\\\\n",
    "\\end{align}\n",
    "so the solution of parameter form is\n",
    "\\begin{cases}\n",
    "x=t^3+t^2\\\\\n",
    "y=\\frac{3}{2}t^2+2t+c\n",
    "\\end{cases}\n",
    "**(2)$(\\frac{\\mathrm d y}{\\mathrm d x})^3-x^3(1-\\frac{\\mathrm d y}{\\mathrm d x})=0$**  \n",
    "**answer:**suppose $\\frac{\\mathrm d y}{\\mathrm d x}=p=tx$  \n",
    "so $(tx)^3-x^3(1-tx)=0$,$x=\\frac{t^3-1}{t}=t^2-\\frac{1}{t}$ then\n",
    "\\begin{align}\n",
    "y&=\\int{p\\mathrm d x}+c\\\\\n",
    "&=\\int{t(t^2-\\frac{1}{t})\\mathrm d (t^2-\\frac{1}{t})}+c\\\\\n",
    "&=\\int{(t^3-1)(2t+\\frac{1}{t^2})\\mathrm d t}+c\\\\\n",
    "&=\\int{(2t^4-t-\\frac{1}{t^2})\\mathrm d t}+c\\\\\n",
    "&=\\frac{2}{5}t^5-\\frac{1}{2}t^2+\\frac{1}{t}+c\\\\\n",
    "\\end{align}\n",
    "so the solution of parameter form is\n",
    "\\begin{cases}\n",
    "x=t^2-\\frac{1}{t}\\\\\n",
    "y=\\frac{2}{5}t^5-\\frac{1}{2}t^2+\\frac{1}{t}+c\n",
    "\\end{cases}\n",
    "**(3)$y=(\\frac{\\mathrm d y}{\\mathrm d x})^2e^{\\frac{\\mathrm d y}{\\mathrm d x}}$**  \n",
    "**answer:**suppose $\\frac{\\mathrm d y}{\\mathrm d x}=p$ then $y=p^2e^p$  \n",
    "so \n",
    "\\begin{align}\n",
    "x&=\\int{\\frac{1}{p}\\mathrm d (p^2e^p)}+c\\\\\n",
    "&=\\int{\\frac{1}{p}(2pe^p+p^2e^p)\\mathrm d p}+c\\\\\n",
    "&=\\int{(2e^p+pe^p)\\mathrm d p}+c\\\\\n",
    "&=(1+p)e^p+c\n",
    "\\end{align}\n",
    "so the solution of parameter form is\n",
    "\\begin{cases}\n",
    "x=(1+p)e^p+c\\\\\n",
    "y=p^2e^p\n",
    "\\end{cases}\n",
    "in addition,$y=0$ is also the solution.  \n",
    "**(4)$y(1+\\frac{\\mathrm d y}{\\mathrm d x})=2a$(\"a\" is a constant.)**  \n",
    "**answer:**suppose $\\frac{\\mathrm d y}{\\mathrm d x}=tan\\phi$ \n",
    "then $y=\\frac{2a}{1+tan^2\\phi}=\\frac{2a}{sec^2\\phi}=2acos^2\\phi$  \n",
    "so\n",
    "\\begin{align}\n",
    "x&=\\int{\\frac{1}{tan\\phi}\\mathrm d (2acos^2\\phi)}+c\\\\\n",
    "&=-4a\\int{cos^2\\phi\\mathrm d \\phi}+c\\\\\n",
    "&=-4a\\int{\\frac{1+cos2\\phi}{2}\\mathrm d \\phi}+c\\\\\n",
    "&=-a(2\\phi+sin2\\phi)+c\n",
    "\\end{align}\n",
    "so the solution of parameter form is\n",
    "\\begin{cases}\n",
    "x=-a(2\\phi+sin2\\phi)+c\\\\\n",
    "y=2acos^2\\phi\n",
    "\\end{cases}\n",
    "**(5)$x^2+(\\frac{\\mathrm d y}{\\mathrm d x})^2=1$**  \n",
    "**answer:**suppose $\\frac{\\mathrm d y}{\\mathrm d x}=cos\\phi$\n",
    "then $x^2+(cos\\phi)^2=1$,$x=\\sqrt{1-cos^2\\phi}=sin\\phi$  \n",
    "so \n",
    "\\begin{align}\n",
    "y&=\\int{cos\\phi\\mathrm d (sin\\phi)}+c\\\\\n",
    "&=\\int{cos^2\\phi\\mathrm d \\phi}+c\\\\\n",
    "&=\\int{\\frac{1+cos2\\phi}{2}\\mathrm d \\phi}+c\\\\\n",
    "&=\\frac{1}{2}\\phi+\\frac{1}{4}sin2\\phi+c\n",
    "\\end{align}\n",
    "so the solution of parameter form is\n",
    "\\begin{cases}\n",
    "x=sin\\phi\\\\\n",
    "y=\\frac{1}{2}\\phi+\\frac{1}{4}sin2\\phi+c\n",
    "\\end{cases}\n",
    "**(6)$y^2(\\frac{\\mathrm d y}{\\mathrm d x}-1)=(2-\\frac{\\mathrm d y}{\\mathrm d x})^2$**  \n",
    "**answer:**suppose $2-\\frac{\\mathrm d y}{\\mathrm d x}=yt$,\n",
    "then $1-\\frac{\\mathrm d y}{\\mathrm d x}=yt-1$,\n",
    "$y=t+\\frac{1}{t}$  \n",
    "so \n",
    "\\begin{align}\n",
    "\\mathrm d x&=\\frac{\\mathrm d y}{y^\\prime}\\\\\n",
    "&=\\frac{t+\\frac{1}{t}}{2-t(t+\\frac{1}{t})}\\\\\n",
    "&=\\frac{(1-t^{-2})\\mathrm d t}{1-t^2}\\\\\n",
    "&=\\frac{t^2-1}{t^2(1-t^2)}\\mathrm d t\\\\\n",
    "&=-\\frac{1}{t^2}\\mathrm d t\n",
    "\\end{align}\n",
    "so $x=\\int{(-\\frac{1}{t^2})\\mathrm d t}+c=\\frac{1}{t}+c$  \n",
    "so the solution of parameter form is\n",
    "\\begin{cases}\n",
    "x=\\frac{1}{t}+c\\\\\n",
    "y=y=t+\\frac{1}{t}\n",
    "\\end{cases}\n",
    "the general solution is $y=\\frac{1}{x-c}+x-c$"
   ]
  },
  {
   "cell_type": "markdown",
   "metadata": {},
   "source": [
    "# <font color='red'>A 26/9"
   ]
  },
  {
   "cell_type": "code",
   "execution_count": null,
   "metadata": {
    "collapsed": true
   },
   "outputs": [],
   "source": []
  }
 ],
 "metadata": {
  "kernelspec": {
   "display_name": "SageMath 7.3",
   "language": "",
   "name": "sagemath"
  },
  "language_info": {
   "codemirror_mode": {
    "name": "ipython",
    "version": 2
   },
   "file_extension": ".py",
   "mimetype": "text/x-python",
   "name": "python",
   "nbconvert_exporter": "python",
   "pygments_lexer": "ipython2",
   "version": "2.7.10"
  }
 },
 "nbformat": 4,
 "nbformat_minor": 0
}
