{
 "cells": [
  {
   "cell_type": "markdown",
   "metadata": {},
   "source": [
    "3.求下列方程的通解：\n",
    "(1)$t^2x''+tx'-x=0;$\n",
    "(2)$t^2x''-4tx'+6x=t;$"
   ]
  },
  {
   "cell_type": "markdown",
   "metadata": {},
   "source": [
    "解(1) 设$x=t^k$，得$k$应满足方程$$k(k-1)+k-1=0$$\n",
    "      即$$k^2-1=0$$\n",
    "      故$$k_1=1,k_2=-1$$\n",
    "      方程的通解为$$x=c_1t+c_2\\frac{1}{t}$$"
   ]
  },
  {
   "cell_type": "markdown",
   "metadata": {},
   "source": [
    "(2)设$x=t^k$，得$k$应满足方程$$k(k-1)-4k+6=0$$\n",
    "   即$$(k-2)(k-3)=0$$\n",
    "   故$$k_1=2,k_2=3$$\n",
    "   方程$t^2x''-4tx'+6x=0$的通解为$$x=c_1t^2+c_2t^3$$\n",
    "   利用常数变易法，求已知方程的形如$$x_1=c_1(t)t^2+c_2(t)t^3$$\n",
    "   的一个特解.\n",
    "   可得$c_1(t)',c_2(t)'$满足\n",
    "   $$\n",
    "   \\begin{cases}\n",
    "   t^2c_1(t)'+t^3c_2(t)'=0\\\\\n",
    "   2tc_1(t)'+3t^2c_2(t)'=\\frac{1}{t}\\\\\n",
    "   \\end{cases}\n",
    "   $$\n",
    "   解得$$c_1(t)'=-\\frac{1}{t^2},c_1(t)=\\frac{1}{t}$$\n",
    "   $$c_2(t)'=\\frac{1}{t^3},c_2(t)=-\\frac{1}{2t^2}$$\n",
    "   故方程的通解为$$x=c_1t^2+c_2t^3+t-\\frac{1}{2}t$$\n",
    "   即$$x=c_1t^2+c_2t^3+\\frac{1}{2}t$$"
   ]
  },
  {
   "cell_type": "markdown",
   "metadata": {
    "collapsed": true
   },
   "source": [
    "# <font color='red'>A  8/11"
   ]
  },
  {
   "cell_type": "code",
   "execution_count": null,
   "metadata": {
    "collapsed": true
   },
   "outputs": [],
   "source": []
  }
 ],
 "metadata": {
  "kernelspec": {
   "display_name": "SageMath 7.3",
   "language": "",
   "name": "sagemath"
  },
  "language_info": {
   "codemirror_mode": {
    "name": "ipython",
    "version": 2
   },
   "file_extension": ".py",
   "mimetype": "text/x-python",
   "name": "python",
   "nbconvert_exporter": "python",
   "pygments_lexer": "ipython2",
   "version": "2.7.10"
  }
 },
 "nbformat": 4,
 "nbformat_minor": 0
}
